x(t) = (1−t)^3 * x0 ​+ 3 * (1−t)^2 * t * x1 ​+ 3 * (1−t) * t^2 * x2 ​ + t^3 * x3
y(t) = (1−t)^3 * y0 ​+ 3 * (1−t)^2 * t * y1 ​+ 3 * (1−t) * t^2 * y2 ​ + t^3 * y3

For points (0, 0), (0, 2), (2, 0), (1, 0) we get

x(t) = (1-t)^3 * 0 + 3 * (1-t)^2 * t * 0 + 3 * (1-t) * t^2 * 2 + t^3 * 1
= 6 * (1-t) * t^2 + t^3 = 6 * t^2 - 6 * t^3 + t^3
= -5 * t^3 + 6 * t^2

y(t) = (1-t)^3 * 0 + 3 * (1-t)^2 * t * 2 + 3 * (1-t) * t^2 * 0 + t^3 * 0
= 6 * (1-t)^2 * t = 6*t - 12 * t^2 + 6 * t^3

so

x(t) = -5 * t^3 + 6 * t^2
y(t) = 6 * t^3 - 12 * t^2 + 6*t